lean/Machines/Machines.lean
@@ -2,7 +2,6 @@
 import Machines.Foundations
 import Machines.Core
 import Machines.Convergent
-import Machines.Live
 import Machines.Refine
 import Machines.LinearMachine
 import Machines.Rewind
